Congruence, narrowing and more

prog-example/fib.c
@@ -1,0 +1,17 @@
+current = 1;
+previous = 1;
+i = 0;
+hey = 2;
+while (i <= 6) {
+	i = i + 1;
+	hey = hey + 18;
+	tmp = previous;
+	previous = current;
+	current = current + tmp;
+};
+while (i <= 16) {
+	i = i + 1;
+	hey = hey + 24;
+};
+x = 100;
+x = x / 7
