AbstractDomain.fst
@@ -3,27 +3,35 @@
 *)
 module AbstractDomain
 
+open PartialOrder
 open DefaultValue
 open FStar.Tactics.Typeclasses
 
 class hasAbstractDomain a = {
+  ab_dom_po: hasPartialOrder a;
   union : a -> a -> a;
   inter : a -> a -> a;
   bottom: a;
   top   : a;
   widen : a -> a -> a;
+  narrow : (l:a) -> (r: a{ab_dom_po.po r l}) -> a;
   assign: string -> a -> a;
   aeq : a -> a -> bool;
+  isBottom : a -> bool;
 }
-let mkAbstractDomain union inter bottom top widen assign aeq
+
+let mkAbstractDomain #a [| hasPartialOrder a |] union inter bottom top widen narrow assign aeq isBottom
     = {
-        union = union
+        ab_dom_po = solve
+      ; union = union
       ; inter = inter
       ; bottom = bottom
       ; top = top
       ; widen = widen
+      ; narrow = narrow
       ; assign = assign
       ; aeq = aeq
+      ; isBottom = isBottom
     }
 
 class hasAbstractOperators a = {
@@ -33,9 +41,10 @@ class hasAbstractOperators a = {
   ; a_op_plus:        a -> a -> a
   ; a_op_minus:       a -> a -> a
   ; a_op_times:       a -> a -> a
+  ; a_op_div:         a -> a -> a
 }
 let mkAbstractOperators #a [| hasAbstractDomain a |] [| hasDefaultValue a |]
-  a_op_unary_minus a_op_plus a_op_minus a_op_times
+  a_op_unary_minus a_op_plus a_op_minus a_op_times a_op_div
   = {
     abstract_domain  = solve
   ; default_value    = solve
@@ -43,6 +52,7 @@ let mkAbstractOperators #a [| hasAbstractDomain a |] [| hasDefaultValue a |]
   ; a_op_plus        = a_op_plus
   ; a_op_minus       = a_op_minus
   ; a_op_times       = a_op_times
+  ; a_op_div         = a_op_div
   }
 
 
@@ -55,7 +65,14 @@ let backward_aop_plus        #a [| hasAbstractOperators a |] [| hasAbstractDomai
     = (x `inter` (r `a_op_minus` y), y `inter` (r `a_op_minus` x)) 
 let backward_aop_minus       #a [| hasAbstractOperators a |] [| hasAbstractDomain a |] (x y r:a)
     = (x `inter` (r `a_op_plus` y), y `inter` (x `a_op_minus` r)) 
-// let backward_aop_mul #a [| hasAbstractOperators a |] [| hasAbstractDomain a |] (x y r:a)
-//     = (x `inter` (r `a_op` y), y `inter` (r `a_op_minus` r))
+let backward_aop_mul #a [| hasAbstractOperators a |] [| hasAbstractDomain a |] (x y r:a)
+     = (x `inter` (r `a_op_div` y), y `inter` (r `a_op_div` x))
 
-// let backward_aop_lt #a [| hasAbstractOperators a |] = 
+open ZeroOrLess
+
+let backward_aop_div #a [| hasZeroOrLess a |] [| hasAbstractOperators a |] [| hasAbstractDomain a |] (x y r:a) =
+    let s = r `a_op_plus` aroundZero
+    in
+     (x `inter` (s `a_op_times` y), y `inter` ((x `a_op_div` s) `union` zeroOnly))
+
+//let backward_aop_lt #a [| hasAbstractOperators a |] = 
