Congruence.fst
@@ -1,0 +1,256 @@
+(*
+@summary: Congruence domain
+*)
+module Congruence
+
+open ExtInt
+open PartialOrder
+open FStar.List.Tot
+open FStar.Tactics.Typeclasses
+open ToString
+
+open AbstractDomain
+open GaloisConnection
+open DefaultValue
+
+open ZeroOrLess
+
+module G = FStar.GSet
+
+type congruence = | SomeCongruence : (a:nat) -> (b:int{if a = 0 then True else (b < a /\ b >= 0)}) -> congruence
+                  | EmptyCongruence : congruence
+
+
+private
+let gbind #a (d:a) (x: congruence) (f: (ne: congruence{SomeCongruence? ne}) -> a) =
+  if SomeCongruence? x then f x else d
+
+module Mul = FStar.Mul
+
+let ( |. ) (x d:int) = if d = 0 then true else let k = x / d in d `Mul.op_Star` k = x
+
+// "a ≡ b [c]" is "a =~ b %% c"
+//let ( %% ) = SomeCongruence
+// is y === x [x']?
+
+let is_in_congruence (x a y: int): bool =
+  if a = 0 then x = y else x % a = y % a
+  //if x = 0 then x' = 1 || x = x' else y % x' = x % x' //y |. abs (x - x')
+// is_in_congruence  0 1 0 (0 === 0 [1] ?) should be true
+
+let lift_const c = SomeCongruence 0 c
+
+let natstar = (x:nat{x > 0})
+
+private
+let test (m:natstar) (x y c:nat) = (
+  is_in_congruence (m `Mul.op_Star` x + c)
+                   m
+                   (m `Mul.op_Star` y + c)
+        )
+
+let ( =~ ) (x: int) (c: congruence) = 
+  match c with
+  | SomeCongruence x' y -> is_in_congruence x x' y
+  | _ -> false
+
+
+let std_gcd (a: int{a <> 0}) (b: int): Tot (n:nat{n <> 0}) =
+  let rec h (a': natstar) (b': nat): Tot (n:natstar) (decreases %[a' + b'; if a' > b' then 0 else 1]) = 
+    if b' = 0 then a'
+    else h b' (a' % b')
+  in h (abs a) (abs b)
+
+let std_lcm (a: int{a <> 0}) (b: int): nat = abs (a `Mul.op_Star` b) / std_gcd a b
+
+let extendZero (f: (v:int{v <> 0}) -> int -> nat) (x y: int) = if x = 0 || y = 0 then 0 else f x y
+
+let gcd (x y:int): nat = if x = 0 then abs y
+                else if y = 0 then abs x
+                else               std_gcd x y
+let lcm = extendZero std_lcm
+
+let includes c1 c2 =
+  let bind = gbind false in
+  c1 <-- c1; c2 <-- c2; let SomeCongruence a b = c1 in let SomeCongruence a' _ = c2 in
+  (a' |. a) && (b =~ c2)
+
+let union' c1 c2 =
+  match c1 with
+    | EmptyCongruence -> c2
+    | SomeCongruence a b -> 
+    ( match c2 with
+      | EmptyCongruence -> c1
+      | SomeCongruence a' b' -> 
+                       let coef = a `gcd` a' `gcd` abs (b - b') in
+                       SomeCongruence
+                                   coef
+                                   (if coef = 0 then 0 else b % coef)
+    )
+
+let union = union'
+
+
+instance _ : hasToString congruence =  { toString = fun i ->  match i with
+  | EmptyCongruence -> "┴"
+  | SomeCongruence a b -> intHasToString.toString b ^ "[" ^ toString a ^ "]"
+}
+
+
+//let x = toString (union' (lift_const 2) (lift_const 18))
+//module Tactics = FStar.Tactics
+//let _ = assert (x == magic ()) by (Tactics.compute (); Tactics.qed ())
+
+let extended_euclidean (a b: int) =
+  let rec h (a b: nat) = 
+	if b = 0 then (a, 1, 0)
+	else match admitP (b << a); (h b (a % b)) with
+		(d, x, y) -> (d, y, x - (a / b) `Mul.op_Star` y)
+  in h (abs a) (abs b)
+
+private
+type neCongr = c:congruence {SomeCongruence? c}
+
+private
+let ( ** ) = Mul.op_Star
+
+private
+let testEGCD x y = let (r,a,b) = extended_euclidean x y in 
+                   (a `Mul.op_Star` x) + (b `Mul.op_Star` y) = r
+
+
+// returns x such that "x = a [a']" and "x = b [b']"
+let solve_two_mod_eq (a a' b b': int) =
+    let (_, a'', b'') = extended_euclidean a' b' in
+    a ** b' ** b'' + b ** a' ** a''
+
+let test_solve_mod a ma b mb = let x = solve_two_mod_eq a ma b mb in
+                                         is_in_congruence x ma a
+                                      && is_in_congruence x mb b
+
+//let _ = assert (test_solve_mod 6 18 2 18) by (Tactics.compute (); Tactics.qed ())
+
+//let solve_two_mod_eq (ac: neCongr) (bc: neCongr) =
+//    let SomeCongruence a a' = ac in let SomeCongruence b b' = bc in
+//    let (_, a'', b'') = extended_euclidean a' b' in
+//    a ** b' ** b'' + b ** a' ** a''
+
+
+//instance congruenceHasPartialOrder : hasPartialOrder congruence = { po = (admit(isPartialOrder gcd); gcd) }
+
+private
+let inter_cong a1 m1 a2 (m2:nat{m1 <> 0 \/ m2 <> 0}) =
+  let g = m1 `gcd` m2 in
+  if is_in_congruence a1 g a2 then (
+    let (_, p, q) = extended_euclidean m1 m2 in
+    let ( * ) = Mul.op_Star in 
+    let x = a1 * m2 / g * q + a2 * m1 / g * p in
+    let m = lcm m1 m2 in  
+    SomeCongruence m (x % (admit (); m))
+  ) else
+    EmptyCongruence
+
+
+//let _ = assert (magic () == lcm  0) by (Tactics.compute (); Tactics.qed ())
+//let _ = assert (magic () = inter_cong 2 3 3 4) by (Tactics.compute (); Tactics.qed ())
+ 
+
+let inter ca cb = 
+  let bind = gbind EmptyCongruence in
+  ca <-- ca; cb <-- cb; let SomeCongruence ma a = ca in let SomeCongruence mb b = cb in
+  if      ma = 1 then (* ca is top *) cb
+  else if mb = 1 then (* cb is top *) ca
+  else if ma = 0 || mb = 0 then
+    (if ca = cb then ca else EmptyCongruence)
+  else    inter_cong a ma b mb
+
+//let _ = assert (inter (mkCong 18 2) (mkCong 19 4) ==magic()) by (Tactics.compute (); Tactics.qed ())
+
+ // let _ = 
+ //   let x = SomeCongruence 3 1 in
+ //   let y = SomeCongruence 4 1 in
+ //   assert (inter x y == magic ()) by (Tactics.compute (); Tactics.qed ())
+   
+   //assert ((solve_two_mod_eq 18 2 18 2 % 18) == magic ()) by (Tactics.compute (); Tactics.qed ())
+//   assert (inter x x == magic ()) by (Tactics.compute (); Tactics.qed ())
+
+
+//let _ = assert (inter x x == magic ()) by (compute (); qed ())
+
+let gamma (i: congruence): GSet.set int = match i with
+  | EmptyCongruence -> GSet.empty
+  | SomeCongruence _ _ -> GSet.comprehend (fun v -> v =~ i)
+
+let values_to_congruence (l: list int) =
+  fold_left union EmptyCongruence (map (fun v -> SomeCongruence 0 v) l)
+  // values [v0, v1, v2, ...]
+  // v_i === a [b]
+  // v_i = k * b + a
+  // v_i - a |. b
+
+//let _ = assert (magic () == values_to_congruence [5;8;12]) by (compute (); qed ())
+
+let mkCong (a:nat) (b:int) = SomeCongruence a (if a = 0 then b else b % a) 
+
+let plus c1 c2 = let bind = gbind EmptyCongruence in
+  c1 <-- c1; c2 <-- c2; let SomeCongruence a b = c1 in let SomeCongruence a' b' = c2 in
+  let a'' = a `gcd` a' in 
+  mkCong a'' (b + b')
+let minus c1 c2 = let bind = gbind EmptyCongruence in
+  c1 <-- c1; c2 <-- c2; let SomeCongruence a b = c1 in let SomeCongruence a' b' = c2 in
+  mkCong (a `gcd` a') (b - b')
+
+let mult c1 c2 = let bind = gbind EmptyCongruence in
+  c1 <-- c1; c2 <-- c2; let SomeCongruence a b = c1 in let SomeCongruence a' b' = c2 in
+  mkCong ((a ** a') `gcd` (a ** b ) `gcd` (a' ** b)) (b ** b')
+
+
+let divide c1 c2 = let bind = gbind EmptyCongruence in
+  c1 <-- c1; c2 <-- c2; let SomeCongruence a b = c1 in let SomeCongruence a' b' = c2 in
+       if a' = 0 && b' = 0
+  then EmptyCongruence
+  else if a' = 0 && not (b' = 0) && (b' |. a) && (b' |. b) then
+       mkCong (a / abs(b')) (b / b')
+  else mkCong 1 0
+
+ 
+let unaryMinus c1 = let bind = gbind EmptyCongruence in
+  c1 <-- c1; let SomeCongruence a b = c1 in  
+  SomeCongruence a (if b = 0 then 0 else (a - b))
+
+let equal (a b:congruence) = a = b
+
+instance _ : hasPartialOrder congruence = { po = (admit (); includes) }
+
+let congruence_alpha set = values_to_congruence (CSet.set_to_list set)
+
+instance _ : hasGaloisConnection int congruence = mkGaloisConnection
+                                 gamma
+                                 (admitP (isMonotonic congruence_alpha); congruence_alpha) (*TODO*)
+                                 (magic ()) 
+
+
+let rec congruence_widen (i j:congruence) =
+  let bind = gbind EmptyCongruence in
+  i <-- i; let SomeCongruence a _ = i in
+  if a = 1 then j else i
+
+instance intervalDomain : hasAbstractDomain congruence = mkAbstractDomain #congruence
+                          union
+                          inter
+           (*bottom*)     EmptyCongruence
+           (*top*)        (SomeCongruence 1 0)
+           (*widen*)      congruence_widen
+                          inter // TODO
+           (*assign*)     (fun _ (i: congruence) -> i)
+                          equal
+                          (fun x -> x = EmptyCongruence)
+                          
+instance _ : hasDefaultValue congruence = {def = top}
+instance _ : hasZeroOrLess congruence = {
+  zeroOrLess = top;
+  zeroOnly   = lift_const 0;
+  aroundZero = lift_const (-1) `union` lift_const 0 `union` lift_const 1 (* which is top *)
+}
+
+instance intervalOperators : hasAbstractOperators congruence = mkAbstractOperators unaryMinus plus minus mult divide
