StaticAnalyser.fst
@@ -14,41 +14,76 @@ open EnumerableMap
 open AbstractDomain
 open ZeroOrLess
 
+module Parser = ToyParser
+
+type mem a = enumerableMap a 
+
+class hasToList a b = {
+  toList: a -> list b 
+}
+instance constHasToList #a: hasToList a a = { toList = fun v -> [v] }
+
+//type isAbstractDomain = (x:Type {exists (d: hasAbstractDomain x). True})
+//open Interval
+// need to express type with behaviour, i.e. existentials types
+//instance tup2HasToList #a: hasToList (a, b) a = { toList = fun v -> [v] }
+
+
+let rec findInTupList #a key (l:list (string * a)): a = admitP (~ (l == [])); match l with
+  | (s,h)::t -> if key = s then h else findInTupList key t  
+
 (* Compute the (abstract) result of an expression *)
 let rec static_analysis_aexp #a [| hasGaloisConnection int a |] [| hasAbstractOperators a |]
                     (st:enumerableMap a)
-                    (exp:lAExp)
+                    (exp:   lAExp      )
+                    //(progs: list (string * list lAExp -> enumerableMap a -> list funDef -> a))
                     : a
-  = let rec h (exp:lAExp): a = 
+  = let rec h (exp:lAExp): a = admitP (~(LAExpCall? exp));
          match exp with
        | LAExpLitt  n       -> alpha' n
        | LAExpVar   varName -> em_get st varName
        | LAExpPlus  a b     -> (h a) `a_op_plus` (h b)
        | LAExpMinus a b     -> (h a) `a_op_minus` (h b)
-       | LAExpMult  a b     ->  (h a) `a_op_times` (h b)
+       | LAExpMult  a b     -> (h a) `a_op_times` (h b)
+       | LAExpDiv   a b     -> (h a) `a_op_div` (h b)
+       //| LAExpCall  v a     -> (let x = findInTupList v )
     in h exp
 
 (* Given an aim and an expression, the following function constraints 
    the variable abstract values present in the expression, using generically
    defined backward operators (see AbstractDomain module) *)
 let rec backward_analysis_aexp #a [| hasGaloisConnection int a |] [| hasAbstractOperators a |]
-                                  [| hasAbstractDomain a |]
+                                  [| hasAbstractDomain a |] [| hasZeroOrLess a |]
                     (st:enumerableMap a)
                     (exp:lAExp)
                     (aim:a)
                     : Tot (enumerableMap a) (decreases exp)
 = let f exp = static_analysis_aexp st exp in
-  match exp with
+  let op2 bop (e1 e2: (x: lAExp{x << exp})) =
+                  (let (aim1, aim2):(tuple2 a a) = bop (f e1) (f e2) aim in (* e1 + e2 should fit in aim *)
+                   let st' = backward_analysis_aexp st e1 aim1 in
+                   backward_analysis_aexp st' e2 aim2)
+  in admitP (~(LAExpCall? exp)); match exp with
   | LAExpLitt n       -> st (* a constant cannot be refined *)
   | LAExpVar  varName -> em_set st varName aim (* TODO: why do I set the value directly? should do some inter or smth *)
-  | LAExpPlus e1 e2   -> let (aim1, aim2):(tuple2 a a) = backward_aop_plus (f e1) (f e2) aim in (* e1 + e2 should fit in aim *)
-                        let st' = backward_analysis_aexp st e1 aim1 in
-                        backward_analysis_aexp st' e2 aim2
-  | LAExpMinus e1 e2  -> let (aim1, aim2):(tuple2 a a) = backward_aop_minus (f e1) (f e2) aim in (* e1 - e1 should fit in aim *)
-                        let st' = backward_analysis_aexp st e1 aim1 in
-                        backward_analysis_aexp st' e2 aim2
-  | LAExpMult a b    ->  st (*todo*)//(h a) `a_op_times` (h b)
+  | LAExpPlus  e1 e2  -> op2 backward_aop_plus  e1 e2
+  | LAExpMinus e1 e2  -> op2 backward_aop_minus e1 e2
+  | LAExpMult  e1 e2  -> op2 backward_aop_mul   e1 e2
+  | LAExpDiv   e1 e2  -> op2 backward_aop_div   e1 e2
+//  | LAExpMult a b    ->  st (*todo*)//(h a) `a_op_times` (h b)
 
+open PartialOrder
+
+let all_bottom #a [| hasAbstractDomain a |] (st: enumerableMap a) = {_em_data = (fun _ -> bottom); _em_keys = st._em_keys}
+
+let is_bottom #a [| hasPartialOrder a |] [| hasAbstractDomain a |] (st: enumerableMap a) =
+    List.Tot.Base.existsb (fun k -> isBottom (em_get st k)) st._em_keys
+
+let spread_bottom #a [| hasPartialOrder a |] [| hasAbstractDomain a |] (st: enumerableMap a) =
+    if is_bottom st
+    then all_bottom st
+    else st
+    
 (* Given an boolean expression `bexp` and a state, `analyse_bexp` returns a state satisfying `bexp` *)
 let rec analyse_bexp #a [| hasAbstractOperators a |] [| hasAbstractDomain a |] [| hasGaloisConnection int a |] [| hasZeroOrLess a |]
                      (st:enumerableMap a)
@@ -56,9 +91,10 @@ let rec analyse_bexp #a [| hasAbstractOperators a |] [| hasAbstractDomain a |] [
                                   (* either the number of non-terminal `not` is decreasing, either
                                      the size of exp (i.e. the deepness of the AST) is decreasing *)
                                   (decreases %[bexp_count_not exp; exp])
-  = match exp with
+  =
+  spread_bottom #a #a_po (match exp with
   | LBExpLitt b -> if b then st (* supposing true doesn't bring anything new *)
-                       else {_em_data = (fun _ -> bottom); _em_keys = st._em_keys} (* variables should all be bottom *)
+                       else all_bottom st (* variables should all be bottom *)
   (* if `not` is terminal (i.e. `! (3 <= 45)`) *)
   | LBExpNot (LBExpEq a b) -> backward_analysis_aexp st (a -. b) (alpha' 0)
   (* otherwise, we apply demorgan and `a <= b ==> b <= a && !(a==b)` *)
@@ -78,39 +114,86 @@ let rec analyse_bexp #a [| hasAbstractOperators a |] [| hasAbstractDomain a |] [
   | LBExpOr   a b -> em_combine (analyse_bexp st a) (analyse_bexp st b) union
   | LBExpEq   a b -> backward_analysis_aexp st (a -. b) (alpha' 0)//lessThanZero
   | LBExpLe   a b -> backward_analysis_aexp st (a -. b) zeroOrLess
+  )
 
 
 open MyIO
 open ToString
 
+let prt str = mi_debug_print_string str
+
+//let _ = assert (Prims.Tot = Tot)
+
 (* This functions perform static analysis on instructions, i.e. on full programs *)
 let rec static_analysis_instr #a [| hasToString a |] [| hasAbstractOperators a |] [| hasAbstractDomain a |] [| hasGaloisConnection int a |] [| hasZeroOrLess a |]
                     (st:enumerableMap a)
-                    (instr:lInstr)
+                    (instr: lInstr)
                     : Tot (enumerableMap a) (decreases instr)
   = let f = static_analysis_instr in
+    let cs (x:enumerableMap a) = emHasToString.toString x in
+    let printCond st c = prt ("\n Cond '" ^ toString c ^ "' gives: \n" ^ cs (analyse_bexp st c)) in
     match instr with
   | LInstrAssign name v -> em_set st name (static_analysis_aexp st v)
   | LInstrSkip          -> st
   | LInstrSeq b1 b2     -> static_analysis_instr (f st b1) b2 
   | LInstrIf c b1 b2    -> let r1 = f (analyse_bexp st     c ) b1 in
                           let r2 = f (analyse_bexp st (!. c)) b2 in
-                          let _ = mi_debug_print_string ("\n Previous state is\n" ^ emHasToString.toString st) in
-                          let _ = mi_debug_print_string ("\n Cond '" ^ toString c ^ "' gives: \n" ^ emHasToString.toString (analyse_bexp st c)) in
-                          let _ = mi_debug_print_string ("\n Cond '" ^ toString (!. c) ^ "' gives: \n" ^ emHasToString.toString (analyse_bexp st (!. c))) in
+                          let _ = prt ("\n [IF] Previous state is\n" ^ cs st) in
+                          let _ = printCond st c in
+                          let _ = printCond st (!. c) in
                           em_combine r1 r2 union
-  | LInstrWhile cond b1 -> let apply_cond st = analyse_bexp st cond in 
+  | LInstrWhile cond body -> let apply_cond st = analyse_bexp st cond in 
+                          let _ = prt ("\n [WHILE] Previous state is\n" ^ cs st) in
+                          //let _ = printCond st c in
                           (* apply_cond takes a state: at each iterations, inveriants 
                              might change, so we need to recompute the condition *)
                           (* TODO: remove that stop parameter *)
+                          let rec unroll (n:nat) st = if n = 0 then st else
+                            (let st = unroll (n-1) st in 
+                             let ifexp = iF cond Then body Else LInstrSkip End in
+                              admitP (ifexp << instr);
+                              static_analysis_instr st ifexp
+                            )
+                          in
+                          let rec findFixPoint state1
+                                               (f: enumerableMap a -> enumerableMap a)
+                                               (stop: option nat)
+                                               : (enumerableMap a) =
+                              let state2 = f state1 in
+                              if em_equal aeq state1 state2 || stop = Some 0
+                              then state2
+                              else (admitP (%[state2] << %[state1]);
+                                    findFixPoint state2 f (match stop with | Some n -> Some (n - 1) | x -> x)) in
                           
-
+                          (*
                           let rec lookForFixPoint current_st (stop: nat): Tot (enumerableMap a) = if stop=0 then current_st else
-                              let new_st  = static_analysis_instr (apply_cond current_st) b1 in (* compute while's body once *)
+                              let _ = prt ("\n [WHILE:LookForFixPoint] state is\n" ^ cs current_st) in
+                              let _ = printCond st cond in
+                              let new_st  = static_analysis_instr (apply_cond current_st) body in (* compute while's body once *)
                               let widened = em_combine new_st (apply_cond (em_combine current_st new_st widen)) union in (* widen the new state *)
                                 if   em_equal aeq current_st widened then widened (* we reached a fixpoint, we're done *)
                                 else lookForFixPoint (admitP (%[widened] << %[current_st]); widened) (stop - 1) in (* TODO: prove some lemma saying widening is ensures termination *)
                           (* we combine the fixpoint state with the old state constrained with the negated condition *)
-                          em_combine (analyse_bexp st (!. cond)) (lookForFixPoint st 4) union
+                          *)
+                          let st = unroll 0 st in
+                          let _ = printCond st (!. cond) in
+                          let unify z = em_combine z (analyse_bexp st (!. cond)) union in
+                          let st' = findFixPoint st (fun x ->
+                              let x' = static_analysis_instr (apply_cond x) body in
+                              em_combine x' (apply_cond (em_combine x x' widen)) union
+                            ) None in
+                          //st'
+                          let st'' = findFixPoint st'
+                                       (fun x -> let y = static_analysis_instr (apply_cond x) body in
+                                              if is_bottom #a #ab_dom_po y then x else y
+                                       )
+                                       (Some 20) in
+                          let _ =  prt ("\n [HEY] st'\n" ^ cs st') in
+                          let _ =  prt ("\n [HEY] st''\n" ^ cs st'') in
+                          let _ =  prt ("\n [HEY] (st'' inter st')\n" ^ cs (em_combine st'' st' inter)) in
+                          //let _ =  prt ("\n [XX] (st'' inter st')\n" ^ cs (em_combine st'' st' inter)) in
+                          unify (em_combine st'' st' inter)
+                          //em_combine (analyse_bexp st (!. cond)) (lookForFixPoint st 4) union
+
 
 
