ToDelete.fst
@@ -1,3 +1,0 @@
-module ToDelete
-
-type matrix #a (#c:nat) (#r:nat) = (list (list a))
